fiat2/src/fiat2/Language.v
@@ -113,6 +113,7 @@ Inductive expr : Type :=
 | ELookup (d k : expr)
 | EOptMatch (e : expr) (e_none : expr) (x : string) (e_some : expr)
 | EDictFold (d e0 : expr) (k v acc : string) (e : expr)
+| ESort (l : expr) (* by value order *)
 (* relational algebra *)
 | EFilter (l : expr) (x : string) (p : expr) (* Select a subset of rows from table *)
 | EJoin (l1 l2 : expr) (x y : string) (p r : expr) (* Join two tables *)
@@ -134,6 +135,7 @@ Section ExprIH.
     (f_lookup : forall d k, P d -> P k -> P (ELookup d k))
     (f_optmatch : forall e e_none x e_some, P e -> P e_none -> P e_some -> P (EOptMatch e e_none x e_some))
     (f_dictfold : forall d e0 k v acc e, P d -> P e0 -> P e -> P (EDictFold d e0 k v acc e))
+    (f_sort : forall l, P l -> P (ESort l))
     (f_filter : forall l x p, P l -> P p -> P (EFilter l x p))
     (f_join : forall l1 l2 x y p r, P l1 -> P l2 -> P p -> P r -> P (EJoin l1 l2 x y p r))
     (f_proj : forall l x r, P l -> P r -> P (EProj l x r)).
@@ -170,6 +172,7 @@ Section ExprIH.
       | ELookup d k => f_lookup d k (expr_IH d) (expr_IH k)
       | EOptMatch e e_none x e_some => f_optmatch e e_none x e_some (expr_IH e) (expr_IH e_none) (expr_IH e_some)
       | EDictFold d e0 k v acc e => f_dictfold d e0 k v acc e (expr_IH d) (expr_IH e0) (expr_IH e)
+      | ESort l => f_sort l (expr_IH l)
       | EFilter l x p => f_filter l x p (expr_IH l) (expr_IH p)
       | EJoin l1 l2 x y p r => f_join l1 l2 x y p r (expr_IH l1) (expr_IH l2) (expr_IH p) (expr_IH r)
       | EProj l x r => f_proj l x r (expr_IH l) (expr_IH r)
